is path predicate

authoring/graphs.dfy
@@ -9,25 +9,34 @@ module GT {
     trait Graph {
         var nodes: set<Node>;
         var edges: set<Edge>;
+        var paths: set<seq<Edge>>;
     }
 
-    class DAG extends Graph {
-        constructor(nodes: set<Node>, edges: set<Edge>)
+    class WeightedDAG extends Graph {
+        constructor(nodes: set<Node>, edges: set<WeightedEdge>, paths: set<seq<WeightedEdge>>)
         requires forall i :: i in edges ==> i.from in nodes && i.to in nodes;
-        // Not recursive.
-        requires forall e :: e in edges ==> !exists j :: j == e.from && j == e.to
+        //requires forall i :: i in paths ==> forall j :: 0 <= j < |i| ==> isPath(edges, i[j])
         {
             this.nodes := nodes;
             this.edges := edges;
+            this.paths := paths;
         }
     }
 
     class WeightedEdge extends Edge {
-        var weight :int;
-        constructor(from: Node, to: Node, weight: int) {
+        var weight :nat;
+        constructor(from: Node, to: Node, weight: nat) {
             this.from := from;
             this.to := to;
             this.weight := weight;
         }
+    }
+
+    predicate isPath(edges: set<WeightedEdge>, subEdges: seq<WeightedEdge>) 
+    reads subEdges
+    requires forall i :: i in subEdges ==> i in edges
+    {
+        forall i :: 0 <= i < |subEdges|-1 ==>
+                subEdges[i].to == subEdges[i+1].from
     }
 }
